start trying calling client1 instead

VST-introduction/verif_client111.v
@@ -81,17 +81,15 @@ Definition kfree1_spec :=
           PROP(
                writable_share sh /\
                is_pointer_or_null original_freelist_pointer /\
-               (Nat.le (S O) (number_structs_available) ) 
+               (Nat.le (S O) (number_structs_available) )  /\ 
+               isptr new_head
                ) 
           PARAMS (new_head) GLOBALS(gv)
           SEP (
-             (if eq_dec new_head nullval then
-              emp 
-              else 
-              (EX v, data_at sh t_run v new_head)) *
-             freelistrep sh n original_freelist_pointer *
-             available sh number_structs_available new_head PGSIZE *
-             (data_at sh t_struct_kmem (Vint (Int.repr xx), original_freelist_pointer) (gv _kmem) )
+                freelistrep sh n original_freelist_pointer *
+                available sh number_structs_available new_head PGSIZE *
+                (data_at sh t_struct_kmem (Vint (Int.repr xx), original_freelist_pointer) (gv _kmem) 
+             )
           )
        POST [ tvoid ]
           PROP(isptr new_head)
@@ -151,12 +149,13 @@ WITH sh : share, new_head:val, original_freelist_pointer:val, xx:Z, gv:globals, 
 PRE [ tptr tvoid ]
     PROP(
         writable_share sh /\
-        is_pointer_or_null new_head /\
+        isptr new_head /\
         (Nat.le (S O) number_structs_available) /\
         ((Nat.eq O n /\ original_freelist_pointer = nullval) \/ (Nat.lt O n /\ isptr original_freelist_pointer))
     ) 
     PARAMS (new_head) GLOBALS(gv)
     SEP (
+        (EX v, data_at sh t_run v new_head) *
         freelistrep sh n original_freelist_pointer *
         available sh number_structs_available new_head PGSIZE *
         data_at sh t_struct_kmem (Vint (Int.repr xx), original_freelist_pointer) (gv _kmem)
@@ -171,13 +170,14 @@ POST [ tptr tvoid ]
             data_at sh t_struct_kmem (Vint (Int.repr xx), original_freelist_pointer) (gv _kmem)
             ).
 
-Definition client2_spec := 
+(*Definition client2_spec := 
     DECLARE _client2
     WITH sh : share, pa1:val, pa2:val, original_freelist_pointer:val, xx:Z, gv:globals, n : nat, next:val, number_structs_available:nat
     PRE [ tptr tvoid, tptr tvoid ]
         PROP(
             writable_share sh /\
-            is_pointer_or_null pa1 /\
+            isptr pa1 /\
+            isptr pa2 /\
             (Nat.le (S (S O)) number_structs_available) /\
             ((Nat.eq O n /\ original_freelist_pointer = nullval) \/ (Nat.lt O n /\ isptr original_freelist_pointer))
         ) 
@@ -203,10 +203,10 @@ Definition client3_spec :=
     PRE [ tptr tvoid, tptr tvoid ]
         PROP(
             writable_share sh /\
-            (*is_pointer_or_null pa1 /\
-            is_pointer_or_null pa2 /\*)
+            isptr pa1 /\
+            isptr pa2 /\
             (Nat.le (S (S O)) number_structs_available) /\
-            ((Nat.eq O n /\ original_freelist_pointer = nullval) \/ (Nat.lt O n /\ isptr original_freelist_pointer))
+            ((Nat.eq O n /\ original_freelist_pointer = nullval) \/ (Nat.lt O n /\ isptr original_freelist_pointer)) 
         ) 
         PARAMS (pa1; pa2) GLOBALS(gv)
         SEP (
@@ -243,6 +243,35 @@ Definition client3_spec :=
                             freelistrep sh n original_freelist_pointer *
                             data_at sh t_struct_kmem (Vint (Int.repr xx), original_freelist_pointer) (gv _kmem)))))
                 )
+                ).*)
+
+Definition client4_spec := 
+    DECLARE _client4
+    WITH sh : share, pa1:val, pa2:val, original_freelist_pointer:val, xx:Z, gv:globals, n : nat, next:val, number_structs_available:nat
+    PRE [ tptr tvoid, tptr tvoid ]
+        PROP(
+            writable_share sh /\
+            isptr pa1 /\
+            isptr pa2 /\
+            (Nat.le (S (S O)) number_structs_available) /\
+            ((Nat.eq O n /\ original_freelist_pointer = nullval) \/ (Nat.lt O n /\ isptr original_freelist_pointer)) 
+        ) 
+        PARAMS (pa1; pa2) GLOBALS(gv)
+        SEP (
+            freelistrep sh n original_freelist_pointer *
+            available sh number_structs_available pa1 PGSIZE *
+            data_at sh t_struct_kmem (Vint (Int.repr xx), original_freelist_pointer) (gv _kmem)
+        )
+    POST [ tptr tvoid ]
+        PROP( )
+            RETURN (pa1) (* we return the head like in the pop function*)
+            SEP 
+            (
+                data_at sh t_run original_freelist_pointer pa1 *
+                data_at sh t_run original_freelist_pointer pa2 *
+                available sh (number_structs_available - 1) (add_offset pa2 PGSIZE) PGSIZE *
+                freelistrep sh n original_freelist_pointer *
+                data_at sh t_struct_kmem (Vint (Int.repr xx), original_freelist_pointer) (gv _kmem)
                 ).
 
 (************************ Gprog  *************************)
@@ -252,7 +281,8 @@ Definition Gprog : funspecs := [
     kalloc1_spec; 
     client1_spec;
     client2_spec;
-    client3_spec
+    client3_spec;
+    client4_spec
 ].
 
 (************************ Proofs  *************************)
@@ -263,10 +293,10 @@ Proof. start_function. Intros. destruct number_structs_available eqn:en; try rep
     - assert (original_freelist_pointer = nullval). {
          rewrite <- H2; auto.
       }
-      rewrite H11. unfold freelistrep. 
-      replace ((S n0) - 1)%nat with n0; try rep_lia.
-      entailer!.
-   - entailer!. assert ((S n0 - 1)%nat = n0); try rep_lia. rewrite H11. entailer.
+      (*rewrite H11.*) unfold freelistrep.
+      rewrite S_pred.
+      entailer.
+   - rewrite S_pred. entailer!. 
 Qed.
 
 Lemma body_kalloc1: semax_body Vprog Gprog f_kalloc1 kalloc1_spec.
@@ -335,9 +365,9 @@ Lemma body_client1: semax_body Vprog Gprog f_client1 client1_spec.
 Proof.
 start_function.
 forward_call (sh, new_head, original_freelist_pointer, xx, gv, n, PGSIZE, number_structs_available). (* call kfree1 *)
-- destruct H as [H1 [H2 [H3 H4]]]; split; auto. destruct H4.
-    + destruct H. rewrite H0. unfold is_pointer_or_null; unfold nullval; simpl; auto.
-    + destruct H. destruct original_freelist_pointer; auto_contradict. unfold is_pointer_or_null; auto.
+- destruct H as [H1 [H2 [H3 H4]]]; split; auto; destruct H4.
+    + destruct H. split; auto. rewrite H0. unfold is_pointer_or_null; unfold nullval; simpl; auto. 
+    + destruct H. split; auto. (*destruct original_freelist_pointer; auto_contradict. unfold is_pointer_or_null; auto.*)
 - forward_call (sh, new_head, xx, (S n), original_freelist_pointer, gv). (* call kalloc *)
     + entailer. unfold freelistrep; fold freelistrep.
         destruct (eq_dec new_head nullval) eqn:enh.
@@ -355,7 +385,8 @@ Lemma body_client2: semax_body Vprog Gprog f_client2 client2_spec.
 Proof.
 start_function.
 forward_call (sh, pa1, original_freelist_pointer, xx, gv, n, PGSIZE, number_structs_available). (* call kfree1 *)
-- destruct H as [H1 [H2 [H3 H4]]]; split; auto. destruct H4; destruct H; auto. rewrite H0; unfold is_pointer_or_null; simpl; auto. 
+- destruct H as [H1 [H2 [H3 H4]]]; split; auto. destruct H4; destruct H; auto.
+    + rewrite H0; unfold is_pointer_or_null; simpl; auto; split; auto. 
     (*+ destruct H. rewrite H0. unfold is_pointer_or_null; unfold nullval; simpl; auto.
     + destruct H. destruct original_freelist_pointer; auto_contradict. unfold is_pointer_or_null; auto.*)
 - forward_call (sh, pa2, pa1, xx, gv, S n, PGSIZE, (number_structs_available -1)%nat). (* call kfree1 *)
@@ -389,22 +420,40 @@ forward_call (sh, pa1, original_freelist_pointer, xx, gv, n, PGSIZE, number_stru
 Admitted.
 
 
+
 Lemma body_client3: semax_body Vprog Gprog f_client3 client3_spec.
 Proof.
 start_function.
+forward_call
+
 forward_call (sh, pa1, original_freelist_pointer, xx, gv, n, PGSIZE, number_structs_available). (* call kfree1 *)
-- destruct (eq_dec pa1 nullval).
-    + entailer!.
-    + EExists. entailer!. admit.
-- admit. (*destruct H as [H1 [H2 [H31 | H32]]]; split; auto. destruct H31; subst; unfold nullval; unfold is_pointer_or_null; simpl; auto.
-    destruct H32. auto. *)
-- forward_call (sh, pa1, xx, (S n), original_freelist_pointer, gv). (* call alloc*)
+- admit. (* should be easy to prove *)
+- forward_call (sh, pa1, xx, (S n), original_freelist_pointer, gv).
     + destruct (eq_dec pa1 nullval) eqn:epa1; try (rewrite S_pred); entailer!.
-    + admit. (*destruct H as [H1 [H2 [H3 H4]]]; split; auto. right; split; try rep_lia; auto.*)
+    + admit. (*EESSY*) (*destruct H as [H1 [H2 [H3 H4]]]; split; auto. right; split; try rep_lia; auto.*)
     + destruct (eq_dec pa1 nullval) eqn:epa1.
         * rewrite e in H0; auto_contradict.
         * forward_call (sh, pa2, original_freelist_pointer, xx, gv, n, PGSIZE, number_structs_available). (* call kfree1 *)
-            -- rewrite S_pred; entailer!.
-    
+        -- rewrite S_pred; entailer!. admit.
+        -- admit.
+        -- forward_call (sh, pa2, xx, (S n), original_freelist_pointer, gv).
+            ++ destruct (eq_dec pa2 nullval) eqn:epa2.
+                entailer!. admit.
+            ++ destruct (eq_dec pa2 nullval) eqn:epa2; entailer!.
+            ++ admit.
+            ++ destruct (eq_dec pa2 nullval) eqn:epa2.
+                ** forward. entailer!. admit. admit.
+                ** forward. entailer!. admit. admit.
+Admitted. 
 
-
+Lemma body_client4: semax_body Vprog Gprog f_client4 client4_spec.
+Proof.
+start_function.
+forward_call (sh, pa1, original_freelist_pointer, xx, gv, n, next, number_structs_available).
+- EExists. entailer!.
+- admit. (* should be easy*)
+-
+ forward_call (sh, pa2, original_freelist_pointer, xx, gv, n, next, number_structs_available).
+    + entailer!. admit.
+    + admit.  (* should be easy*)
+    + forward. entailer!.
